dist with hacl-star

steel/dist/hacl-star-v0.3.0/gcc-compatible/EverCrypt_DRBG.d
@@ -1,0 +1,15 @@
+./EverCrypt_DRBG.o EverCrypt_DRBG.d : EverCrypt_DRBG.c EverCrypt_DRBG.h \
+ evercrypt_targetconfig.h libintvector.h \
+ ../kremlin/include/kremlin/internal/types.h \
+ ../kremlin/include/kremlin/lowstar_endianness.h \
+ ../kremlin/kremlib/dist/minimal/fstar_uint128_gcc64.h \
+ ../kremlin/kremlib/dist/minimal/FStar_UInt128.h \
+ ../kremlin/include/kremlin/internal/compat.h \
+ ../kremlin/include/kremlin/internal/target.h \
+ ../kremlin/include/kremlin/internal/callconv.h \
+ ../kremlin/kremlib/dist/minimal/FStar_UInt_8_16_32_64.h \
+ ../kremlin/kremlib/dist/minimal/LowStar_Endianness.h EverCrypt_HMAC.h \
+ Hacl_Kremlib.h Hacl_HMAC.h Hacl_Impl_Blake2_Constants.h Hacl_Hash.h \
+ Hacl_Blake2s_32.h Lib_Memzero0.h Hacl_Blake2b_32.h Hacl_Spec.h \
+ EverCrypt_Hash.h Vale.h EverCrypt_AutoConfig2.h \
+ Lib_RandomBuffer_System.h Hacl_HMAC_DRBG.h Hacl_Lib.h
