steel/dist/hacl-star-v0.3.0/gcc-compatible/Hacl_Streaming_SHA2.d
@@ -1,0 +1,13 @@
+./Hacl_Streaming_SHA2.o Hacl_Streaming_SHA2.d : Hacl_Streaming_SHA2.c Hacl_Streaming_SHA2.h \
+ evercrypt_targetconfig.h libintvector.h \
+ ../kremlin/include/kremlin/internal/types.h \
+ ../kremlin/include/kremlin/lowstar_endianness.h \
+ ../kremlin/kremlib/dist/minimal/fstar_uint128_gcc64.h \
+ ../kremlin/kremlib/dist/minimal/FStar_UInt128.h \
+ ../kremlin/include/kremlin/internal/compat.h \
+ ../kremlin/include/kremlin/internal/target.h \
+ ../kremlin/include/kremlin/internal/callconv.h \
+ ../kremlin/kremlib/dist/minimal/FStar_UInt_8_16_32_64.h \
+ ../kremlin/kremlib/dist/minimal/LowStar_Endianness.h Hacl_Kremlib.h \
+ Hacl_Hash.h Hacl_Blake2s_32.h Lib_Memzero0.h \
+ Hacl_Impl_Blake2_Constants.h Hacl_Blake2b_32.h Hacl_Spec.h
